Split code in modules

Compiler.dfy
@@ -8,476 +8,260 @@
   (a small subset of the Java Virtual Machine) and proves that this
   compiler preserves the semantics of the source programs. */
 
-/* * 1. The virtual machine. */
+include "Definitions.dfy"
+include "Lists.dfy"
+include "Sequences.dfy"
 
-/* The machine operates on a code [c] (a fixed list of instructions)
-  and three variable components:
-- a program counter, denoting a position in [c]
-- a state assigning integer values to variables
-- an evaluation stack, containing integers.
-*/
+module Compiler {
 
-/* The instruction set of the machine. */
+  import opened Definitions
+  import opened Lists
+  import opened Sequences
 
-datatype option<T> = Some(T) | None
-datatype list<T> = Nil | Cons(T, list<T>)
-type id = string
+  /* * 3. IMP programs whose free variables are in [U]. */
 
-// My append function (Leroy uses Coq lists)
-function append<T>(l1: list<T>, l2: list<T>): list<T>
-{
-  match l1
-  case Nil => l2
-  case Cons(x, xs) => Cons(x, append(xs, l2))
-}
+  /* We redefine the abstract syntax of IMP to ensure that all
+    variables mentioned in the program are taken from [U]. */
 
-// My length function
-function length<T>(l: list<T>): nat
-{
-  match l
-  case Nil => 0
-  case Cons(_, xs) => 1 + length(xs)
-}
+  const U': set<id>
+  const vx := "X"
+  const vy := "Y"
+  const U: set<id> := {vx, vy} + U'
+  type Uvar = x: id | x in U witness vx
 
-datatype instruction =
-  | Iconst(nat)
-  | Ivar(id)
-  | Isetvar(id)
-  | Iadd
-  | Isub
-  | Imul
-  | Ibranch_forward(nat)
-  | Ibranch_backward(nat)
-  | Ibeq(nat)
-  | Ibne(nat)
-  | Ible(nat)
-  | Ibgt(nat)
-  | Ihalt
+  datatype aexp =
+    | ANum(nat)
+    | AId (Uvar)        /*r <--- NEW */
+    | APlus(aexp, aexp)
+    | AMinus(aexp, aexp)
+    | AMult(aexp, aexp)
 
-type code = list<instruction>
+  datatype bexp =
+    | BTrue
+    | BFalse
+    | BEq(aexp, aexp)
+    | BLe(aexp, aexp)
+    | BNot(bexp)
+    | BAnd(bexp, bexp)
 
-/* [code_at(C, pc) = Some i] if [i] is the instruction at position [pc]
-  in the list of instructions [C]. */
+  datatype com =
+    | CSkip
+    | CAss(Uvar, aexp)   /*r <--- NEW */
+    | CSeq(com, com)
+    | CIf(bexp, com, com)
+    | CWhile(bexp, com)
 
-function code_at (C: code, pc: nat) : option<instruction>
-{
-  match (C, pc)
-  case (Nil, _)         => None
-  case (Cons(i, _), 0)  => Some(i)
-  case (Cons(_, C'), n) => code_at(C', n - 1)
-}
+  /* The code for an arithmetic expression [a]
+  - executes in sequence (no branches)
+  - deposits the value of [a] at the top of the stack
+  - preserves the variable state.
+  This is the familiar translation to "reverse Polish notation".
+  */
 
-type stack = list<nat>
-
-/* A state maps atoms to natural numbers*/
-type state = map<id, nat>
-
-/* The semantics of the virtual machine is given in small-step style,
-  as a transition relation between machine configuration: triples
-  (program counter, evaluation stack, variable state).
-  The transition relation is parameterized by the code [c].
-  There is one transition rule for each kind of instruction,
-  except [Ihalt], which has no transition. */
-
-type configuration = (nat, stack, state)
-
-// A difference between defining inductive datatype in Coq and least predicate
-// is that in the inductive case, we're forced to think about the relationships
-// between all arguments, whereas here, we might forget to include a relationship
-// in the conjunction.
-least predicate transition (C: code, conf1: configuration, conf2: configuration)
-{
-  var (pc1, stk1, st1) := conf1;
-  var (pc2, stk2, st2) := conf2;
-  match code_at(C, pc1)
-  case Some(Iconst(n)) =>
-      && pc2 == pc1 + 1
-      && stk2 == Cons(n, stk1)
-      && st2 == st1
-  case Some(Ivar(x)) =>
-      && pc2 == pc1 + 1
-      && x in st1 // TODO: this is different from Leroy
-      && stk2 == Cons(st1[x], stk1)
-      && st2 == st1
-  case Some(Isetvar(x)) =>
-      exists v ::
-      && pc2 == pc1 + 1
-      && stk1 == Cons(v, stk2)
-      && st2 == st1[x:=v]
-  case Some(Iadd) =>
-      exists v1, v2, vs ::
-      && pc2 == pc1 + 1
-      && stk1 == Cons(v2, Cons(v1, vs))
-      && stk2 == Cons(v1 + v2, vs)
-      && st1 == st2
-  case Some(Isub) =>
-      exists v1, v2, vs ::
-      && pc2 == pc1 + 1
-      && stk1 == Cons(v2, Cons(v1, vs))
-      && stk2 == Cons(v1 - v2, vs)
-      && st1 == st2
-  case Some(Imul) =>
-      exists v1, v2, vs ::
-      && pc2 == pc1 + 1
-      && stk1 == Cons(v2, Cons(v1, vs))
-      && stk2 == Cons(v1 * v2, vs)
-      && st1 == st2
-  case Some(Ibranch_forward(ofs)) =>
-      && pc2 == pc1 + 1 + ofs
-      && stk1 == stk2
-      && st1 == st2
-  case Some(Ibranch_backward(ofs)) =>
-      && pc1 + 1 > ofs
-      && pc2 == pc1 + 1 - ofs
-      && stk1 == stk2
-      && st1 == st2
-  case Some(Ibeq(ofs)) =>
-      exists v1, v2 ::
-      && stk1 == Cons(v2, Cons(v1, stk2))
-      && (if v1 == v2 then pc2 == pc1 + 1 - ofs else pc2 == pc1 + 1)
-      && st1 == st2
-  case Some(Ibne(ofs)) =>
-      exists v1, v2 ::
-      && stk1 == Cons(v2, Cons(v1, stk2))
-      && (if v1 == v2 then pc2 == pc1 + 1 else pc2 == pc1 + 1 + ofs)
-      && st1 == st2
-  case Some(Ible(ofs)) =>
-      exists v1, v2 ::
-      && stk1 == Cons(v2, Cons(v1, stk2))
-      && (if v1 < v2 then pc2 == pc1 + 1 + ofs else pc2 == pc1 + 1)
-      && st1 == st2
-  case Some(Ibgt(ofs)) =>
-      exists v1, v2 ::
-      && stk1 == Cons(v2, Cons(v1, stk2))
-      && (if v1 < v2 then pc2 == pc1 + 1 else pc2 == pc1 + 1 + ofs)
-      && st1 == st2
-  case Some(Ihalt) => false
-  case None => false
-}
-
-// To avoid working with higher-order functions, rather than defining a star relation,
-// I will follow the example of the NipkovKlein-chapter7.dfy file and define
-// a specialized reflexive, transitive closure relation for the transition predicate.
-
-/* Zero, one or several transitions: reflexive, transitive closure of */
-// transition
-least predicate star_transition(C: code, confA: configuration, confC: configuration)
-{
-  || confA == confC
-  || exists confB :: transition(C, confA, confB) && star_transition(C, confB, confC)
-}
-
-/* As usual with small-step semantics, we form sequences of machine transitions
-  to define the behavior of a code.  We always start with [pc = 0]
-  and an empty evaluation stack.  We stop successfully if [pc] points
-  to an [Ihalt] instruction and the evaluation stack is empty.
-*/
-predicate mach_terminates (C: code, s_init: state, s_fin: state)
-{
-  exists pc ::
-  && code_at(C, pc) == Some(Ihalt)
-  && star_transition(C, (0, Nil, s_init), (pc, Nil, s_fin))
-}
-
-greatest predicate infseq_transition(C: code, conf: configuration)
-{
-  exists conf2 :: transition(C, conf, conf2) && infseq_transition(C, conf2)
-}
-
-predicate mach_diverges(C: code, s_init: state)
-{
-  infseq_transition(C, (0, Nil, s_init))
-}
-
-predicate irred_transition(C: code, conf: configuration)
-{
-  forall conf2 :: !(transition(C, conf, conf2))
-}
-
-/* A third case can occur: after a finite number of transitions,
-  the machine hits a configuration where it cannot make any transition,
-  and this state is not a final configuration ([Ihalt] instruction and empty stack).
-  In this case, we say that the machine "goes wrong", which is
-  a politically-correct way of saying that our program just crashed. */
-
-predicate mach_goes_wrong(C: code, s_init: state)
-{
-  exists pc, stk, s_fin ::
-  && star_transition(C, (0, Nil, s_init), (pc, stk, s_fin))
-  && irred_transition(C, (pc, stk, s_fin))
-  && (code_at(C, pc) != Some(Ihalt) || stk != Nil)
-}
-
-/* An important property of the virtual machine is that it is deterministic:
-  from a given configuration, it can transition to at most one other configuration. */
-
-lemma machine_deterministic(C: code, conf: configuration, conf1: configuration, conf2: configuration)
-  requires transition(C, conf, conf1)
-  requires transition(C, conf, conf2)
-  ensures  conf1 == conf2
-{}
-
-/* As a consequence of this determinism, it follows that
-  the final state of a terminating program is unique,
-  and that a program cannot both terminate and diverge,
-  or terminate and go wrong, or diverge and go wrong.
-  These results follow from the generic determinism properties */
-
-lemma stop_irred(C: code, pc: nat, stk: stack, st: state)
-  requires code_at(C, pc) == Some(Ihalt)
-  ensures irred_transition(C, (pc, stk, st))
-{}
-
-// TODO do other predicates have to be least here? I might want to experiment with removing the "least" and see what happens
-
-least lemma finseq_unique(C: code, a: configuration, c: configuration, c': configuration)
-  requires star_transition(C, a, c) && irred_transition(C, c)
-  requires star_transition(C, a, c') && irred_transition(C, c')
-  ensures c == c'
-{
-  if a != c && a != c'
+  function compile_aexp (a: aexp) : code
   {
-    var b :| transition(C, a, b) && star_transition(C, b, c);
-    var b' :| transition(C, a, b') && star_transition(C, b', c');
-    machine_deterministic(C, a, b, b');
+    match a
+    case ANum(n) => Cons(Iconst(n), Nil)
+    case AId(v) => Cons(Ivar(v), Nil)
+    case APlus(a1, a2) => append(compile_aexp(a1), append(compile_aexp(a2), Cons(Iadd, Nil)))
+    case AMinus(a1, a2) => append(compile_aexp(a1), append(compile_aexp(a2), Cons(Isub, Nil)))
+    case AMult(a1, a2) => append(compile_aexp(a1), append(compile_aexp(a2), Cons(Imul, Nil)))
   }
-}
 
-lemma terminates_unique(C: code, st: state, st1: state, st2: state)
-  requires mach_terminates(C, st, st1)
-  requires mach_terminates(C, st, st2)
-  ensures st1 == st2
-{
-  var pc1 :| code_at(C, pc1) == Some(Ihalt) && star_transition(C, (0, Nil, st), (pc1, Nil, st1));
-  var pc2 :| code_at(C, pc2) == Some(Ihalt) && star_transition(C, (0, Nil, st), (pc2, Nil, st2));
-  finseq_unique(C, (0, Nil, st), (pc1, Nil, st1), (pc2, Nil, st2));
-}
+  /* Some examples. */
 
-lemma terminates_goeswrong_exclusive(C: code, st: state, st': state)
-  requires mach_terminates(C, st, st')
-  ensures !mach_goes_wrong(C, st)
-{
-  var pc :| code_at(C, pc) == Some(Ihalt) && star_transition(C, (0, Nil, st), (pc, Nil, st'));
-  var conf := (0, Nil, st);
-  var conf' := (pc, Nil, st');
-  forall stk_stuck, st_stuck, pc_stuck
-    | && star_transition(C, (0, Nil, st), (pc_stuck, stk_stuck, st_stuck))
-      && irred_transition(C, (pc_stuck, stk_stuck, st_stuck))
-    ensures && pc == pc_stuck
-            && stk_stuck == Nil
-            {
-              finseq_unique(C, conf, conf', (pc_stuck, stk_stuck, st_stuck));
-            }
-}
+  method example1()
+  {
+    var e1 := compile_aexp(APlus(AId(vx), ANum(1)));
+    var expected1 := Cons(Ivar(vx), Cons(Iconst(1), Cons(Iadd, Nil)));
+    assert e1 == expected1;
 
-least lemma infseq_star_inv(C: code, a: configuration, c: configuration)
-  requires star_transition(C, a, c)
-  requires infseq_transition(C, a)
-  ensures infseq_transition(C, c)
-{
-  if a != c {
-    var b :| && transition(C, a, b)
-             && star_transition(C, b, c);
-    forall b' | transition(C, a, b') ensures b == b' {
-      machine_deterministic(C, a, b, b');
+    var e2 := compile_aexp(AMult(AId(vy), APlus(AId(vx), ANum(1))));
+    var expected2 := Cons(Ivar(vy), Cons(Ivar(vx), Cons(Iconst(1), Cons(Iadd, Cons(Imul, Nil)))));
+    assert e2 == expected2;
+  }
+
+  function compile_bexp(b: bexp, cond: bool, ofs: nat) : code
+  {
+    match b
+    case BTrue =>
+        if cond then Cons(Ibranch_forward(ofs), Nil) else Nil
+    case BFalse =>
+        if cond then Nil else Cons(Ibranch_forward(ofs), Nil)
+    case BEq(a1, a2) =>
+        append(compile_aexp(a1), append(compile_aexp(a2), if cond then Cons(Ibeq(ofs), Nil) else Cons(Ibne(ofs), Nil)))
+    case BLe(a1, a2) =>
+        append(compile_aexp(a1), append(compile_aexp(a2), if cond then Cons(Ible(ofs), Nil) else Cons(Ibgt(ofs), Nil)))
+    case BNot(b1) =>
+        compile_bexp(b1, !cond, ofs)
+    case BAnd(b1, b2) =>
+        var c2 := compile_bexp(b2, cond, ofs);
+        var c1 := compile_bexp(b1, false, if cond then length(c2) else ofs + length(c2));
+        append(c1, c2)
+  }
+
+  /* Examples. */
+
+  method example2()
+  {
+    var e1 := compile_bexp(BEq(AId(vx), ANum(1)), true, 42);
+    var expected1 := Cons(Ivar(vx), Cons(Iconst(1), Cons(Ibeq(42), Nil)));
+    assert e1 == expected1;
+
+    var e2 := compile_bexp(BAnd(BLe(ANum(1), AId(vx)), BLe(AId(vx), ANum(10))), false, 42);
+    var expected2 := Cons(Iconst(1), Cons(Ivar(vx), Cons(Ibgt(45), Cons(Ivar(vx), Cons(Iconst(10), Cons(Ibgt(42), Nil))))));
+    assert e2 == expected2;
+
+    var e3 := compile_bexp(BNot(BAnd(BTrue, BFalse)), true, 42);
+    var expected3 := Cons(Ibranch_forward(42), Nil);
+    assert e3 == expected3;
+  }
+
+  /* The code for a command [c]
+  - updates the variable state as prescribed by [c]
+  - preserves the stack
+  - finishes on the next instruction immediately following the generated code.
+  Again, see slides for explanations of the generated branch offsets.
+  */
+
+  // Remark: notations are a nice thing in Coq
+  function compile_com(c: com) : code
+  {
+    match c
+    case CSkip =>
+        Nil
+    case CAss(id, a) =>
+        append(compile_aexp(a), Cons(Isetvar(id), Nil))
+    case CSeq(c1, c2) =>
+        append(compile_com(c1), compile_com(c2))
+    case CIf(b, ifso, ifnot) =>
+        var code_ifso := compile_com(ifso);
+        var code_ifnot := compile_com(ifnot);
+        append(compile_bexp(b, false, length(code_ifso) + 1),
+              append(code_ifso,
+                      Cons(Ibranch_forward(length(code_ifnot)),
+                          code_ifnot)))
+    case CWhile(b, body) =>
+        var code_body := compile_com(body);
+        var code_test := compile_bexp(b, false, length(code_body) + 1);
+        append(code_test,
+              append(code_body,
+                      Cons(Ibranch_backward(length(code_test) + length(code_body) + 1),
+                          Nil)))
+  }
+
+  /* The code for a program [p] (a command) is similar, but terminates
+    cleanly on an [Ihalt] instruction. */
+
+  function compile_program(p: com): code
+  {
+    append(compile_com(p), Cons(Ihalt, Nil))
+  }
+
+  /* Examples of compilation. */
+
+  method example3()
+  {
+    var e1 := compile_program(CAss(vx, APlus(AId(vx), ANum(1))));
+    var expected1 := Cons(Ivar(vx), Cons(Iconst(1), Cons(Iadd, Cons(Isetvar(vx), Cons(Ihalt, Nil)))));
+    assert e1 == expected1;
+
+    var e2 := compile_program(CWhile(BTrue, CSkip));
+    var expected2 := Cons(Ibranch_backward(1), Cons(Ihalt, Nil));
+    assert e2 == expected2;
+
+    var e3 := compile_program(CIf(BEq(AId(vx), ANum(1)), CAss(vx, ANum(0)), CSkip));
+    var expected3 := Cons(Ivar(vx), Cons(Iconst(1), Cons(Ibne(3), Cons(Iconst(0), Cons(Isetvar(vx), Cons(Ibranch_forward(0), Cons(Ihalt, Nil)))))));
+    assert e3 == expected3; 
+  }
+
+  /* 3. Semantic preservation */
+
+  /* Auxiliary results about code sequences. */
+
+  /* To reason about the execution of compiled code, we need to consider
+    code sequences [C2] that are at position [pc] in a bigger code
+    sequence [C = C1 ++ C2 ++ C3].  The following predicate
+    [codeseq_at C pc C2] does just this. */
+
+  least predicate codeseq_at(C: code, pc: nat, C2: code)
+  {
+    exists C1, C3 :: pc == length(C1) && C == append(C1, append(C2, C3))
+  }
+
+  /* We show a number of no-brainer lemmas about [code_at] and [codeseq_at],
+    then populate a "hint database" so that Coq can use them automatically. */
+
+  // I'm concerned about the effect this will have on the Dafny proof:
+  // the fact that we can't have a hint database.
+
+  lemma code_at_app(i: instruction, c2: code, c1: code, pc: nat)
+    requires pc == length(c1)
+    ensures code_at(append(c1, Cons(i, c2)), pc) == Some(i)
+  {}
+
+  lemma codeseq_at_head(C: code, pc: nat, i: instruction, C': code)
+  requires codeseq_at(C, pc, Cons(i, C'))
+  ensures code_at(C, pc) == Some(i)
+  {
+    forall C1, C3
+    | pc == length(C1) && C == append(C1, append(Cons(i, C'), C3))
+    {
+      code_at_app(i, append(C', C3), C1, pc);
     }
   }
-}
 
-lemma irred_not_infseq(C: code, a: configuration)
-requires irred_transition(C, a)
-ensures !infseq_transition(C, a)
-{}
+  // Another difference with Coq: no type inference; function signatures have to be written in full
+  // One more difference: arguments to lemmas have to be passed explicitly
 
-lemma infseq_finseq_excl(C: code, a: configuration, c: configuration)
-  requires star_transition(C, a, c)
-  requires irred_transition(C, c)
-  ensures !infseq_transition(C, a)
-{
-  if a != c {
-    if infseq_transition(C, a) {
-      infseq_star_inv(C, a, c);
+  lemma codeseq_at_tail(C: code, pc: nat, i: instruction, C': code)
+  requires codeseq_at(C, pc, Cons(i, C'))
+  ensures codeseq_at(C, pc + 1, C')
+  {
+    forall C1, C3
+        | pc == length(C1) && C == append(C1, append(Cons(i, C'), C3))
+        ensures codeseq_at(C, pc + 1, C')
+    {
+      var C1' := append(C1, Cons(i, Nil));
+      assert pc + 1 == length(C1');
+      assert C == append(C1', append(C', C3));
     }
   }
+
+  // Lemma codeseq_at_tail:
+  //   forall C pc i C',
+  //   codeseq_at C pc (i :: C') ->
+  //   codeseq_at C (pc + 1) C'.
+  // Proof.
+  //   intros. inversion H. 
+  //   change (C1 ++ (i :: C') ++ C3)
+  //     with (C1 ++ (i :: nil) ++ C' ++ C3).
+  //   rewrite <- app_ass. constructor. rewrite app_length. auto.
+  // Qed. 
+
+  // Lemma codeseq_at_app_left:
+  //   forall C pc C1 C2,
+  //   codeseq_at C pc (C1 ++ C2) ->
+  //   codeseq_at C pc C1.
+  // Proof.
+  //   intros. inversion H. rewrite app_ass. constructor. auto.
+  // Qed.
+
+  // Lemma codeseq_at_app_right:
+  //   forall C pc C1 C2,
+  //   codeseq_at C pc (C1 ++ C2) ->
+  //   codeseq_at C (pc + length C1) C2.
+  // Proof.
+  //   intros. inversion H. rewrite app_ass. rewrite <- app_ass. constructor. rewrite app_length. auto.
+  // Qed.
+
+  // Lemma codeseq_at_app_right2:
+  //   forall C pc C1 C2 C3,
+  //   codeseq_at C pc (C1 ++ C2 ++ C3) ->
+  //   codeseq_at C (pc + length C1) C2.
+  // Proof.
+  //   intros. inversion H. repeat rewrite app_ass. rewrite <- app_ass. constructor. rewrite app_length. auto.
+  // Qed.
+
+  // Hint Resolve codeseq_at_head codeseq_at_tail codeseq_at_app_left codeseq_at_app_right codeseq_at_app_right2: codeseq.
 }
-
-lemma terminates_diverges_exclusive(C: code, st: state, st': state)
-  requires mach_terminates(C, st, st')
-  ensures !mach_diverges(C, st)
-{
-  var pc :| code_at(C, pc) == Some(Ihalt) && star_transition(C, (0, Nil, st), (pc, Nil, st'));
-  var conf := (0, Nil, st);
-  var conf' := (pc, Nil, st');
-  infseq_finseq_excl(C, conf, conf');
-}
-
-lemma goeswrong_diverges_exclusive(C: code, st: state)
-  requires mach_goes_wrong(C, st)
-  ensures !mach_diverges(C, st)
-{
-  var conf := (0, Nil, st);
-  var pc, stk, s_fin :|
-    && star_transition(C, conf, (pc, stk, s_fin))
-    && irred_transition(C, (pc, stk, s_fin))
-    && (code_at(C, pc) != Some(Ihalt) || stk != Nil);
-  var conf' := (pc, stk, s_fin);
-  infseq_finseq_excl(C, conf, conf');
-}
-
-/* * 3. IMP programs whose free variables are in [U]. */
-
-/* We redefine the abstract syntax of IMP to ensure that all
-  variables mentioned in the program are taken from [U]. */
-
-const U': set<id>
-const vx := "X"
-const vy := "Y"
-const U: set<id> := {vx, vy} + U'
-type Uvar = x: id | x in U witness vx
-
-datatype aexp =
-  | ANum(nat)
-  | AId (Uvar)        /*r <--- NEW */
-  | APlus(aexp, aexp)
-  | AMinus(aexp, aexp)
-  | AMult(aexp, aexp)
-
-datatype bexp =
-  | BTrue
-  | BFalse
-  | BEq(aexp, aexp)
-  | BLe(aexp, aexp)
-  | BNot(bexp)
-  | BAnd(bexp, bexp)
-
-datatype com =
-  | CSkip
-  | CAss(Uvar, aexp)   /*r <--- NEW */
-  | CSeq(com, com)
-  | CIf(bexp, com, com)
-  | CWhile(bexp, com)
-
-/* The code for an arithmetic expression [a]
-- executes in sequence (no branches)
-- deposits the value of [a] at the top of the stack
-- preserves the variable state.
-This is the familiar translation to "reverse Polish notation".
-*/
-
-function compile_aexp (a: aexp) : code
-{
-  match a
-  case ANum(n) => Cons(Iconst(n), Nil)
-  case AId(v) => Cons(Ivar(v), Nil)
-  case APlus(a1, a2) => append(compile_aexp(a1), append(compile_aexp(a2), Cons(Iadd, Nil)))
-  case AMinus(a1, a2) => append(compile_aexp(a1), append(compile_aexp(a2), Cons(Isub, Nil)))
-  case AMult(a1, a2) => append(compile_aexp(a1), append(compile_aexp(a2), Cons(Imul, Nil)))
-}
-
-/* Some examples. */
-
-method example1()
-{
-  var e1 := compile_aexp(APlus(AId(vx), ANum(1)));
-  var expected1 := Cons(Ivar(vx), Cons(Iconst(1), Cons(Iadd, Nil)));
-  assert e1 == expected1;
-
-  var e2 := compile_aexp(AMult(AId(vy), APlus(AId(vx), ANum(1))));
-  var expected2 := Cons(Ivar(vy), Cons(Ivar(vx), Cons(Iconst(1), Cons(Iadd, Cons(Imul, Nil)))));
-  assert e2 == expected2;
-}
-
-function compile_bexp(b: bexp, cond: bool, ofs: nat) : code
-{
-  match b
-  case BTrue =>
-      if cond then Cons(Ibranch_forward(ofs), Nil) else Nil
-  case BFalse =>
-      if cond then Nil else Cons(Ibranch_forward(ofs), Nil)
-  case BEq(a1, a2) =>
-      append(compile_aexp(a1), append(compile_aexp(a2), if cond then Cons(Ibeq(ofs), Nil) else Cons(Ibne(ofs), Nil)))
-  case BLe(a1, a2) =>
-      append(compile_aexp(a1), append(compile_aexp(a2), if cond then Cons(Ible(ofs), Nil) else Cons(Ibgt(ofs), Nil)))
-  case BNot(b1) =>
-      compile_bexp(b1, !cond, ofs)
-  case BAnd(b1, b2) =>
-      var c2 := compile_bexp(b2, cond, ofs);
-      var c1 := compile_bexp(b1, false, if cond then length(c2) else ofs + length(c2));
-      append(c1, c2)
-}
-
-/* Examples. */
-
-method example2()
-{
-  var e1 := compile_bexp(BEq(AId(vx), ANum(1)), true, 42);
-  var expected1 := Cons(Ivar(vx), Cons(Iconst(1), Cons(Ibeq(42), Nil)));
-  assert e1 == expected1;
-
-  var e2 := compile_bexp(BAnd(BLe(ANum(1), AId(vx)), BLe(AId(vx), ANum(10))), false, 42);
-  var expected2 := Cons(Iconst(1), Cons(Ivar(vx), Cons(Ibgt(45), Cons(Ivar(vx), Cons(Iconst(10), Cons(Ibgt(42), Nil))))));
-  assert e2 == expected2;
-
-  var e3 := compile_bexp(BNot(BAnd(BTrue, BFalse)), true, 42);
-  var expected3 := Cons(Ibranch_forward(42), Nil);
-  assert e3 == expected3;
-}
-
-/* The code for a command [c]
-- updates the variable state as prescribed by [c]
-- preserves the stack
-- finishes on the next instruction immediately following the generated code.
-Again, see slides for explanations of the generated branch offsets.
-*/
-
-// Remark: notations are a nice thing in Coq
-function compile_com(c: com) : code
-{
-  match c
-  case CSkip =>
-      Nil
-  case CAss(id, a) =>
-      append(compile_aexp(a), Cons(Isetvar(id), Nil))
-  case CSeq(c1, c2) =>
-      append(compile_com(c1), compile_com(c2))
-  case CIf(b, ifso, ifnot) =>
-      var code_ifso := compile_com(ifso);
-      var code_ifnot := compile_com(ifnot);
-      append(compile_bexp(b, false, length(code_ifso) + 1),
-             append(code_ifso,
-                    Cons(Ibranch_forward(length(code_ifnot)),
-                         code_ifnot)))
-  case CWhile(b, body) =>
-      var code_body := compile_com(body);
-      var code_test := compile_bexp(b, false, length(code_body) + 1);
-      append(code_test,
-             append(code_body,
-                    Cons(Ibranch_backward(length(code_test) + length(code_body) + 1),
-                         Nil)))
-}
-
-/* The code for a program [p] (a command) is similar, but terminates
-  cleanly on an [Ihalt] instruction. */
-
-function compile_program(p: com): code
-{
-  append(compile_com(p), Cons(Ihalt, Nil))
-}
-
-/* Examples of compilation. */
-
-method example3()
-{
-  var e1 := compile_program(CAss(vx, APlus(AId(vx), ANum(1))));
-  var expected1 := Cons(Ivar(vx), Cons(Iconst(1), Cons(Iadd, Cons(Isetvar(vx), Cons(Ihalt, Nil)))));
-  assert e1 == expected1;
-
-  var e2 := compile_program(CWhile(BTrue, CSkip));
-  var expected2 := Cons(Ibranch_backward(1), Cons(Ihalt, Nil));
-  assert e2 == expected2;
-
-  var e3 := compile_program(CIf(BEq(AId(vx), ANum(1)), CAss(vx, ANum(0)), CSkip));
-  var expected3 := Cons(Ivar(vx), Cons(Iconst(1), Cons(Ibne(3), Cons(Iconst(0), Cons(Isetvar(vx), Cons(Ibranch_forward(0), Cons(Ihalt, Nil)))))));
-  assert e3 == expected3; 
-}
-
