Definitions.dfy
@@ -1,0 +1,146 @@
+// A Dafny implementation of Xavier Leroy's compiler-verification Coq exercises,
+// which were offered to students of the Deepspec Summer School 2017.
+// The exercises can be found in https://github.com/DeepSpec/dsss17/blob/master/compiler/Compiler.v.
+// All subsequent comments enclosed in /*...*/ are taken verbatim from the exercises.
+// The single-line comments (starting with //) are for my notes.
+
+// This module defines the main data types that are used in the compiler.
+
+/* This chapter defines a compiler from the Imp language to a virtual machine
+  (a small subset of the Java Virtual Machine) and proves that this
+  compiler preserves the semantics of the source programs. */
+
+include "Lists.dfy"
+
+module Definitions {
+  
+  import opened Lists
+
+  /* * 1. The virtual machine. */
+
+  /* The machine operates on a code [c] (a fixed list of instructions)
+    and three variable components:
+  - a program counter, denoting a position in [c]
+  - a state assigning integer values to variables
+  - an evaluation stack, containing integers.
+  */
+
+  /* The instruction set of the machine. */
+  type id = string
+
+  datatype instruction =
+    | Iconst(nat)
+    | Ivar(id)
+    | Isetvar(id)
+    | Iadd
+    | Isub
+    | Imul
+    | Ibranch_forward(nat)
+    | Ibranch_backward(nat)
+    | Ibeq(nat)
+    | Ibne(nat)
+    | Ible(nat)
+    | Ibgt(nat)
+    | Ihalt
+
+  type code = list<instruction>
+
+  /* [code_at(C, pc) = Some i] if [i] is the instruction at position [pc]
+    in the list of instructions [C]. */
+
+  function code_at (C: code, pc: nat) : option<instruction>
+  {
+    match (C, pc)
+    case (Nil, _)         => None
+    case (Cons(i, _), 0)  => Some(i)
+    case (Cons(_, C'), n) => code_at(C', n - 1)
+  }
+
+  type stack = list<nat>
+
+  /* A state maps atoms to natural numbers*/
+  type state = map<id, nat>
+
+  /* The semantics of the virtual machine is given in small-step style,
+    as a transition relation between machine configuration: triples
+    (program counter, evaluation stack, variable state).
+    The transition relation is parameterized by the code [c].
+    There is one transition rule for each kind of instruction,
+    except [Ihalt], which has no transition. */
+
+  type configuration = (nat, stack, state)
+
+  // A difference between defining inductive datatype in Coq and least predicate
+  // is that in the inductive case, we're forced to think about the relationships
+  // between all arguments, whereas here, we might forget to include a relationship
+  // in the conjunction.
+  least predicate transition (C: code, conf1: configuration, conf2: configuration)
+  {
+    var (pc1, stk1, st1) := conf1;
+    var (pc2, stk2, st2) := conf2;
+    match code_at(C, pc1)
+    case Some(Iconst(n)) =>
+        && pc2 == pc1 + 1
+        && stk2 == Cons(n, stk1)
+        && st2 == st1
+    case Some(Ivar(x)) =>
+        && pc2 == pc1 + 1
+        && x in st1 // TODO: this is different from Leroy
+        && stk2 == Cons(st1[x], stk1)
+        && st2 == st1
+    case Some(Isetvar(x)) =>
+        exists v ::
+        && pc2 == pc1 + 1
+        && stk1 == Cons(v, stk2)
+        && st2 == st1[x:=v]
+    case Some(Iadd) =>
+        exists v1, v2, vs ::
+        && pc2 == pc1 + 1
+        && stk1 == Cons(v2, Cons(v1, vs))
+        && stk2 == Cons(v1 + v2, vs)
+        && st1 == st2
+    case Some(Isub) =>
+        exists v1, v2, vs ::
+        && pc2 == pc1 + 1
+        && stk1 == Cons(v2, Cons(v1, vs))
+        && stk2 == Cons(v1 - v2, vs)
+        && st1 == st2
+    case Some(Imul) =>
+        exists v1, v2, vs ::
+        && pc2 == pc1 + 1
+        && stk1 == Cons(v2, Cons(v1, vs))
+        && stk2 == Cons(v1 * v2, vs)
+        && st1 == st2
+    case Some(Ibranch_forward(ofs)) =>
+        && pc2 == pc1 + 1 + ofs
+        && stk1 == stk2
+        && st1 == st2
+    case Some(Ibranch_backward(ofs)) =>
+        && pc1 + 1 > ofs
+        && pc2 == pc1 + 1 - ofs
+        && stk1 == stk2
+        && st1 == st2
+    case Some(Ibeq(ofs)) =>
+        exists v1, v2 ::
+        && stk1 == Cons(v2, Cons(v1, stk2))
+        && (if v1 == v2 then pc2 == pc1 + 1 - ofs else pc2 == pc1 + 1)
+        && st1 == st2
+    case Some(Ibne(ofs)) =>
+        exists v1, v2 ::
+        && stk1 == Cons(v2, Cons(v1, stk2))
+        && (if v1 == v2 then pc2 == pc1 + 1 else pc2 == pc1 + 1 + ofs)
+        && st1 == st2
+    case Some(Ible(ofs)) =>
+        exists v1, v2 ::
+        && stk1 == Cons(v2, Cons(v1, stk2))
+        && (if v1 < v2 then pc2 == pc1 + 1 + ofs else pc2 == pc1 + 1)
+        && st1 == st2
+    case Some(Ibgt(ofs)) =>
+        exists v1, v2 ::
+        && stk1 == Cons(v2, Cons(v1, stk2))
+        && (if v1 < v2 then pc2 == pc1 + 1 else pc2 == pc1 + 1 + ofs)
+        && st1 == st2
+    case Some(Ihalt) => false
+    case None => false
+  }
+}
