Sequences.dfy
@@ -1,0 +1,183 @@
+// A Dafny implementation of Xavier Leroy's Sequences module,
+// which defines helper lemmas for his compiler-verification exercises.
+// https://github.com/DeepSpec/dsss17/blob/master/compiler/Sequences.v
+// All subsequent comments enclosed in /*...*/ are taken verbatim from the exercises.
+// The single-line comments (starting with //) are for my notes.
+
+// To avoid working with higher-order functions, rather than defining a star relation,
+// I will follow the example of the NipkovKlein-chapter7.dfy file and define
+// a specialized reflexive, transitive closure relation for the transition predicate.
+
+include "Definitions.dfy"
+include "Lists.dfy"
+
+module Sequences {
+
+  import opened Definitions
+  import opened Lists
+
+  /* Zero, one or several transitions: reflexive, transitive closure of */
+  // transition
+  least predicate star_transition(C: code, confA: configuration, confC: configuration)
+  {
+    || confA == confC
+    || exists confB :: transition(C, confA, confB) && star_transition(C, confB, confC)
+  }
+
+  /* As usual with small-step semantics, we form sequences of machine transitions
+    to define the behavior of a code.  We always start with [pc = 0]
+    and an empty evaluation stack.  We stop successfully if [pc] points
+    to an [Ihalt] instruction and the evaluation stack is empty.
+  */
+  predicate mach_terminates (C: code, s_init: state, s_fin: state)
+  {
+    exists pc ::
+    && code_at(C, pc) == Some(Ihalt)
+    && star_transition(C, (0, Nil, s_init), (pc, Nil, s_fin))
+  }
+
+  greatest predicate infseq_transition(C: code, conf: configuration)
+  {
+    exists conf2 :: transition(C, conf, conf2) && infseq_transition(C, conf2)
+  }
+
+  predicate mach_diverges(C: code, s_init: state)
+  {
+    infseq_transition(C, (0, Nil, s_init))
+  }
+
+  predicate irred_transition(C: code, conf: configuration)
+  {
+    forall conf2 :: !(transition(C, conf, conf2))
+  }
+
+  /* A third case can occur: after a finite number of transitions,
+    the machine hits a configuration where it cannot make any transition,
+    and this state is not a final configuration ([Ihalt] instruction and empty stack).
+    In this case, we say that the machine "goes wrong", which is
+    a politically-correct way of saying that our program just crashed. */
+
+  predicate mach_goes_wrong(C: code, s_init: state)
+  {
+    exists pc, stk, s_fin ::
+    && star_transition(C, (0, Nil, s_init), (pc, stk, s_fin))
+    && irred_transition(C, (pc, stk, s_fin))
+    && (code_at(C, pc) != Some(Ihalt) || stk != Nil)
+  }
+
+  /* An important property of the virtual machine is that it is deterministic:
+    from a given configuration, it can transition to at most one other configuration. */
+
+  lemma machine_deterministic(C: code, conf: configuration, conf1: configuration, conf2: configuration)
+    requires transition(C, conf, conf1)
+    requires transition(C, conf, conf2)
+    ensures  conf1 == conf2
+  {}
+
+  /* As a consequence of this determinism, it follows that
+    the final state of a terminating program is unique,
+    and that a program cannot both terminate and diverge,
+    or terminate and go wrong, or diverge and go wrong.
+    These results follow from the generic determinism properties */
+
+  lemma stop_irred(C: code, pc: nat, stk: stack, st: state)
+    requires code_at(C, pc) == Some(Ihalt)
+    ensures irred_transition(C, (pc, stk, st))
+  {}
+
+  // TODO do other predicates have to be least here? I might want to experiment with removing the "least" and see what happens
+
+  least lemma finseq_unique(C: code, a: configuration, c: configuration, c': configuration)
+    requires star_transition(C, a, c) && irred_transition(C, c)
+    requires star_transition(C, a, c') && irred_transition(C, c')
+    ensures c == c'
+  {
+    if a != c && a != c'
+    {
+      var b :| transition(C, a, b) && star_transition(C, b, c);
+      var b' :| transition(C, a, b') && star_transition(C, b', c');
+      machine_deterministic(C, a, b, b');
+    }
+  }
+
+  lemma terminates_unique(C: code, st: state, st1: state, st2: state)
+    requires mach_terminates(C, st, st1)
+    requires mach_terminates(C, st, st2)
+    ensures st1 == st2
+  {
+    var pc1 :| code_at(C, pc1) == Some(Ihalt) && star_transition(C, (0, Nil, st), (pc1, Nil, st1));
+    var pc2 :| code_at(C, pc2) == Some(Ihalt) && star_transition(C, (0, Nil, st), (pc2, Nil, st2));
+    finseq_unique(C, (0, Nil, st), (pc1, Nil, st1), (pc2, Nil, st2));
+  }
+
+  lemma terminates_goeswrong_exclusive(C: code, st: state, st': state)
+    requires mach_terminates(C, st, st')
+    ensures !mach_goes_wrong(C, st)
+  {
+    var pc :| code_at(C, pc) == Some(Ihalt) && star_transition(C, (0, Nil, st), (pc, Nil, st'));
+    var conf := (0, Nil, st);
+    var conf' := (pc, Nil, st');
+    forall stk_stuck, st_stuck, pc_stuck
+      | && star_transition(C, (0, Nil, st), (pc_stuck, stk_stuck, st_stuck))
+        && irred_transition(C, (pc_stuck, stk_stuck, st_stuck))
+      ensures && pc == pc_stuck
+              && stk_stuck == Nil
+              {
+                finseq_unique(C, conf, conf', (pc_stuck, stk_stuck, st_stuck));
+              }
+  }
+
+  least lemma infseq_star_inv(C: code, a: configuration, c: configuration)
+    requires star_transition(C, a, c)
+    requires infseq_transition(C, a)
+    ensures infseq_transition(C, c)
+  {
+    if a != c {
+      var b :| && transition(C, a, b)
+              && star_transition(C, b, c);
+      forall b' | transition(C, a, b') ensures b == b' {
+        machine_deterministic(C, a, b, b');
+      }
+    }
+  }
+
+  lemma irred_not_infseq(C: code, a: configuration)
+  requires irred_transition(C, a)
+  ensures !infseq_transition(C, a)
+  {}
+
+  lemma infseq_finseq_excl(C: code, a: configuration, c: configuration)
+    requires star_transition(C, a, c)
+    requires irred_transition(C, c)
+    ensures !infseq_transition(C, a)
+  {
+    if a != c {
+      if infseq_transition(C, a) {
+        infseq_star_inv(C, a, c);
+      }
+    }
+  }
+
+  lemma terminates_diverges_exclusive(C: code, st: state, st': state)
+    requires mach_terminates(C, st, st')
+    ensures !mach_diverges(C, st)
+  {
+    var pc :| code_at(C, pc) == Some(Ihalt) && star_transition(C, (0, Nil, st), (pc, Nil, st'));
+    var conf := (0, Nil, st);
+    var conf' := (pc, Nil, st');
+    infseq_finseq_excl(C, conf, conf');
+  }
+
+  lemma goeswrong_diverges_exclusive(C: code, st: state)
+    requires mach_goes_wrong(C, st)
+    ensures !mach_diverges(C, st)
+  {
+    var conf := (0, Nil, st);
+    var pc, stk, s_fin :|
+      && star_transition(C, conf, (pc, stk, s_fin))
+      && irred_transition(C, (pc, stk, s_fin))
+      && (code_at(C, pc) != Some(Ihalt) || stk != Nil);
+    var conf' := (pc, stk, s_fin);
+    infseq_finseq_excl(C, conf, conf');
+  }
+}
